SteelUtils: some cleaning + fixing build
moving helpers to lib_misc/SeqUtils,
removing useless helpers

lib_misc/SeqUtils.fst
@@ -1,6 +1,32 @@
 module SeqUtils
 
+module L = FStar.List.Tot
 module U32 = FStar.UInt32
+
+let rec lemma_seq_to_list_append (#a:Type) (s1 s2: Seq.seq a)
+  : Lemma
+  (ensures
+    Seq.seq_to_list (Seq.append s1 s2) == L.append (Seq.seq_to_list s1) (Seq.seq_to_list s2))
+  (decreases Seq.length s1)
+  = if Seq.length s1 = 0 then (assert (Seq.append s1 s2 `Seq.equal` s2))
+    else (
+      let s1' = Seq.slice s1 1 (Seq.length s1) in
+      let s12 = Seq.append s1 s2 in
+      let s12' = Seq.slice s12 1 (Seq.length s12) in
+      lemma_seq_to_list_append s1' s2;
+      assert (s12' `Seq.equal` Seq.append s1' s2)
+    )
+
+// remove SMTPat
+let lemma_index_slice (#a:Type) (s:Seq.seq a)
+  (i:nat)
+  (j:nat{i <= j /\ j <= Seq.length s})
+  (k:nat{k < j - i})
+  : Lemma
+  (requires True)
+  (ensures (Seq.index (Seq.slice s i j) k == Seq.index s (k + i)))
+  =
+  Seq.lemma_index_slice s i j k
 
 noextract
 let init_nat (len: nat)
