src/SteelUtils.fst
@@ -12,61 +12,6 @@ let starl (l: list vprop)
   =
   L.fold_right star l emp
 
-
-let rec partition_equiv_filter (#a: Type) (f: a -> Tot bool) (l: list a)
-  : Lemma
-  (L.partition f l == (L.filter f l, L.filter (fun x -> not (f x)) l))
-  = match l with
-  | [] -> ()
-  | hd::tl -> partition_equiv_filter f tl
-
-let rec count_equiv_filter (#a: eqtype) (l: list a) (x: a)
-  : Lemma
-  (ensures L.count x l = L.length (L.filter (fun y -> y = x) l))
-  (decreases l)
-  = match l with
-  | [] -> ()
-  | hd::tl -> count_equiv_filter tl x
-
-let rec filter_equiv (#a: Type) (l: list a) (f1 f2: a -> Tot bool)
-  : Lemma
-  (requires forall x. f1 x = f2 x)
-  (ensures L.filter f1 l == L.filter f2 l)
-  (decreases l)
-  = match l with
-  | [] -> ()
-  | hd::tl -> filter_equiv tl f1 f2
-
-
-let filter_lemma (#a: eqtype) (l: list a) (x: a)
-  : Lemma
-  (requires L.count x l == 1)
-  (ensures ([x], L.filter (fun y -> y <> x) l) == L.partition (fun y -> y = x) l)
-  =
-  let f = fun y -> y = x in
-  let r = L.partition f l in
-  partition_equiv_filter f l;
-  L.partition_count f l x;
-  assert (L.count x l == L.count x (fst r) + L.count x (snd r));
-  assert (1 == L.count x (fst r) + L.count x (snd r));
-  assert (L.count x (fst r) = 1 || L.count x (snd r) = 1);
-  if (L.count x (snd r) = 1) then (
-    L.mem_count (snd r) x;
-    L.mem_memP x (snd r);
-    assert (L.memP x (snd r));
-    L.mem_filter (fun x -> not (f x)) (snd r) x;
-    assert (not (f x));
-    assert (f x)
-  );
-  assert (L.count x (fst r) = 1);
-  count_equiv_filter l x;
-  assert (L.length (fst r) = 1);
-  L.mem_count (fst r) x;
-  assert (L.mem x (fst r));
-  assert (fst r = [x]);
-  filter_equiv l (fun y -> not (y = x)) (fun y -> y <> x)
-
-
 let rec starl_append (l1 l2: list vprop)
   : Lemma
   (starl (L.append l1 l2) `equiv` (starl l1 `star` starl l2))
@@ -100,54 +45,6 @@ let rec starl_append (l1 l2: list vprop)
         (hd `star` (starl tl `star` starl l2))
         (starl l1 `star` starl l2)
 
-
-
-let starl_singleton (#a: Type) (f: a -> Tot vprop) (l: list a)
-  : Lemma
-  (requires L.length l == 1)
-  (ensures starl (L.map f l) `equiv` f (L.hd l))
-  =
-  assert (l == [L.hd l]);
-  assert (L.map f l == [f (L.hd l)]);
-  let p1 = starl (L.map f l) in
-  let p3 = f (L.hd l) in
-  let p2 = p3 `star` emp in
-  assert (starl [f (L.hd l)] == f (L.hd l) `star` emp);
-  equiv_refl p1;
-  assert (p1 `equiv` p2);
-  cm_identity p3;
-  assert ((emp `star` p3) `equiv` p3);
-  star_commutative emp p3;
-  assert ((emp `star` p3) `equiv` p2);
-  equiv_sym (emp `star` p3) p2;
-  equiv_trans
-    p2
-    (emp `star` p3)
-    p3;
-  assert (p2 `equiv` p3);
-  equiv_trans p1 p2 p3
-
-let starl_append_hd_map (#a: Type) (f: a -> vprop) (l: list a) (x: a)
-  : Lemma
-  (starl (L.map f (x::l)) `equiv` (f x `star` starl (L.map f l)))
-  =
-  let p0 = starl (L.map f (x::l)) in
-  let p1 = starl (L.map f l) in
-  L.map_append f [x] l;
-  assert (L.map f (x::l) == L.append (L.map f [x]) (L.map f l));
-  starl_append (L.map f [x]) (L.map f l);
-  assert (p0 `equiv` (starl (L.map f [x]) `star` p1));
-  starl_singleton f [x];
-  assert (starl (L.map f [x]) `equiv` f x);
-  equiv_refl p1;
-  star_congruence
-    (starl (L.map f [x])) p1
-    (f x) p1;
-  equiv_trans
-    p0
-    (starl (L.map f [x]) `star` p1)
-    (f x `star` p1)
-
 let starl_seq (s: Seq.seq vprop)
   : vprop
   =
@@ -159,7 +56,7 @@ let starl_seq_append (s1 s2: Seq.seq vprop)
   =
   let l1 = Seq.seq_to_list s1 in
   let l2 = Seq.seq_to_list s2 in
-  Utils.lemma_seq_to_list_append s1 s2;
+  SeqUtils.lemma_seq_to_list_append s1 s2;
   starl_append l1 l2
 
 let starl_seq_unpack (s: Seq.seq vprop) (n: nat)
